Splinter/Betree/LinkedBetreeRefinement.i.dfy
@@ -12,7 +12,75 @@ module LinkedBetreeRefinement {
   import opened Buffers
   import GenericDisk
   import opened BoundedPivotsLib
-  import opened LinkedBetree
+  import opened LinkedBetreeMod
+  import opened StampedMod
+  import PivotBetree
 
+  function EmptyStampedBetree() : StampedBetree
+  {
+    Stamped(LinkedBetree(None, DiskView(map[])), 0)
+  }
 
+  function ILbl(lbl: TransitionLabel) : PivotBetree.TransitionLabel
+  {
+    match lbl
+      case QueryLabel(endLsn, key, value) => PivotBetree.QueryLabel(endLsn, key, value)
+      case PutLabel(puts) => PivotBetree.PutLabel(puts)
+      case QueryEndLsnLabel(endLsn) => PivotBetree.QueryEndLsnLabel(endLsn)
+      case FreezeAsLabel(stampedBetree) => PivotBetree.FreezeAsLabel(
+        if stampedBetree.value.WF()
+        then IStampedBetree(stampedBetree)
+        else IStampedBetree(EmptyStampedBetree())
+      )
+      case InternalLabel() => PivotBetree.InternalLabel()
+  }
+
+  function IChildren(linked: LinkedBetree) : seq<PivotBetree.BetreeNode>
+    requires linked.WF()
+    requires linked.HasRoot()
+  {
+    var numChildren := |linked.Root().children|;
+    seq(numChildren, i requires 0<=i<numChildren => ILinkedBetree(linked.ChildAtIdx(i)))
+  }
+
+  function ILinkedBetree(linked: LinkedBetree) : PivotBetree.BetreeNode
+    requires linked.WF()
+  {
+    if linked.root.None?
+    then PivotBetree.Nil
+    else
+      var node := linked.Root();
+      PivotBetree.BetreeNode(node.buffers, node.pivotTable, IChildren(linked))
+  }
+
+  function IStampedBetree(stampedBetree: StampedBetree) : PivotBetree.StampedBetree
+    requires stampedBetree.value.WF()
+  {
+    Stamped(ILinkedBetree(stampedBetree.value), stampedBetree.seqEnd)
+  }
+
+  function I(v: Variables) : PivotBetree.Variables
+    requires v.WF()
+  {
+    PivotBetree.Variables(v.memtable, ILinkedBetree(v.linked))
+  }
+
+  predicate Inv(v: Variables)
+  {
+    true  // TODO!
+  }
+
+  lemma InitRefines(v: Variables, stampedBetree: StampedBetree)
+    requires Init(v, stampedBetree)
+    ensures PivotBetree.Init(I(v), IStampedBetree(stampedBetree))
+  {
+  }
+
+  lemma NextRefines(v: Variables, v': Variables, lbl: TransitionLabel)
+    requires Inv(v)
+    requires Next(v, v', lbl)
+    ensures v'.WF()
+    ensures PivotBetree.Next(I(v), I(v'), ILbl(lbl))
+  {
+  }
 }
